## 11. Nov 25

a) $\frac{1}{2} + \frac{1}{3} = \frac{5}{6}$
b) $\frac{x}{y} + \frac{a}{b} = \frac{xb + ya}{yb}$
c) $\frac{1}{a} \cdot \frac{1}{a^2} \cdot a^3 + \frac{a}{b} = \frac{a}{b} + 1$
d)$\frac{1}{1 + \frac{1}{1 - \frac{1}{1+x}}}= \frac{x}{1+2x}$
e) $\frac{a}{b} - \frac{b}{a} = \frac{a^2 - b^2}{ab}$

## 24. Nov 25

a)
$(A \cup B) \cap (A \cup \overline{B})$
$= (A \cap A) \cup (A \cap \overline{B}) \cup (B \cap A) \cup (B \cap \overline{B})$
$= A \cup (A \cap \overline{B}) \cup (B \cap A)$ Absorptionsgesetz
$= A \cup (A \cap B)$
$=A$


b)
$(A \cap B) \cup (A \cap \overline{B})$
$= ((A \cap B) \cup A) \cap ((A \cap B) \cup \overline{B})$
$= A \cap ((A \cap B) \cup \overline{B})$
$= (A \cap (A \cap B) \cup (A \cap \overline{B}))$
$= (A \cap A \cap B) \cup (A \cap \overline{B})$
$= (A \cap B) \cup (A \cap \overline{B})$
$= (A \cup A) \cap (A \cup \overline{B}) \cap (B \cup A) \cap (B \cup \overline{B})$ ab hier
$= A \cap (A \cup \overline{B}) \cup (B \cup A)$
$= A \cup (B \cup A)$
$= A$

c)
$\overline{\overline{A} \cup B}$
$=A \cup \overline{B}$
$= A$

d) Hilfe
$= (A \cup B) \cap (\overline{A} \cup C)$
$= (A \cap \overline{A}) \cup (A \cap C) \cup (B \cap \overline{A}) \cup (B \cap C)$
$= (A \cap C) \cup (B \cap \overline{A}) \cup (B \cap C)$
$= (A \cap C) \cup (B \cap C)$
$= (A \cup B) \cap (A \cup C) \cap (C \cup B) \cap C$
$= (A \cap B \cap C) \cap (A \cap B \cap C)$
$= A \cap B \cap C$


e)
$(A \cup B) \cap (A \cap \overline{A})$
$= (A \cup B) \cap \varnothing$
$= \varnothing$

f)
$\overline{A \cap B} \cup (A \cup B)$
$= (\overline{A} \cup \overline{B}) \cup (A \cup B)$
$= \overline{A} \cup A \cup B \cup \overline{B}$
$= \Omega$

g)
$A \cap ((B \cup C) \cup \overline{B})$
$= A \cap \Omega$
$= A$

h)
$(A \cap B) \cup (A \cap \overline{B}) \cup (\overline{A} \cap B)$
$=(A \cap (A \cup \overline{B}) \cap (B \cup A) \cap \Omega) \cup (\overline{A} \cap B)$
$=(A \cap (B \cup A)) \cup (\overline{A} \cap B)$
$=A \cup (\overline{A} \cap B)$
$= A \cup B$

i)
$(A \cap B) \cap (\overline{A} \cup \overline{B})$
$(A \cap B) \cap \overline{A \cap B}$
$= \varnothing$

j)
$\overline{\overline{(A \cup B)} \cup C}$
$=(A \cup B) \cap \overline{C}$

k) hilfe
$(A \cap (B \cup C)) \cup (\overline{A} \cap B \cap C)$
$=((A \cap B) \cup (A \cap C)) \cup (\overline{A} \cap B \cap C)$
$=(A \cap (A \cup C) \cap (B \cup A) \cap (B \cup C)) \cup (\overline{A} \cap B \cap C)$
$=(A \cap B \cap C) \cup (\overline{A} \cap B \cap C)$

